proved wf_reborrow after reborrow_stack

Rustv/Rustv.thy
@@ -365,6 +365,10 @@ lemma wf_tags_spec:
 proof (induction ts)
 qed auto
 
+lemma wf_tags_snoc:
+  "wf_tags (ts @ [stack]) \<longleftrightarrow> wf_tags ts \<and> wf_reborrow stack \<and> stack_finite stack"
+  using wf_tags_spec by auto
+
 lemma list_update_forall:
   "\<lbrakk>\<forall>x \<in> set xs. P x; P x'\<rbrakk> \<Longrightarrow> \<forall>x \<in> set (xs[p := x']). P x"
   using set_update_subset_insert by fastforce
@@ -453,21 +457,24 @@ fun wf_heap :: "'a globals_ram_scheme \<Rightarrow> bool" where
     \<and> wf_tags (tags s)
     \<and> collect_tags (tags s) \<subseteq> set (issued_tags s)"
 
+fun pop_tags_stack :: "tag \<Rightarrow> (ref_kind * tag set) stack \<Rightarrow> (ref_kind * tag set) stack" where
+  "pop_tags_stack t stack = dropWhile (\<lambda>entry. t \<notin> snd entry) stack"
+
 fun pop_tags :: "tagged_ref \<Rightarrow> 'a globals_ram_scheme \<Rightarrow> 'a globals_ram_scheme" where
   "pop_tags r s =
     (let p = the_ptr (pointer r);
          stack = tags s ! p;
-         stack' = dropWhile (\<lambda>entry. (tag r) \<notin> snd entry) stack in
+         stack' = pop_tags_stack (tag r) stack in
     s\<lparr> tags := (tags s)[p := stack'] \<rparr>)"
 
 fun_cases pop_tags_elims: "pop_tags r s = s'"
 
 lemma hd_dropWhile_stack:
   assumes
-    "dropWhile (\<lambda>entry. (tag r) \<notin> snd entry) stack = stack'"
+    "pop_tags_stack (tag r) stack = stack'"
     "\<exists>entry \<in> set stack. (tag r) \<in> snd entry"
   shows "tag r \<in> snd (hd stack')"
-  by (metis assms(1) assms(2) dropWhile_eq_Nil_conv hd_dropWhile)
+  by (metis assms(1) assms(2) pop_tags_stack.simps dropWhile_eq_Nil_conv hd_dropWhile)
 
 lemma dropWhile_stack_reborrow:
   "wf_reborrow stack \<and> dropWhile P stack \<noteq> [] \<Longrightarrow> wf_reborrow (dropWhile P stack)"
@@ -647,23 +654,15 @@ lemma writable_stack_the_index:
   shows "\<exists>!i. i < length stack \<and> t \<in> snd (stack ! i)"
   using wf_reborrow_tag_position_unique writable_stack_in_collect_tags assms by simp
 
-
-
-lemma writable_stack_pop_tags_nonempty:
-  assumes
-    "pop_tags r s = s'"
-    "the_ptr (pointer r) < length (tags s)"
-    "writable_stack (tag r) ((tags s) ! the_ptr (pointer r))"
-  shows "(tags s') ! the_ptr (pointer r) \<noteq> []"
-  sorry
-
-lemma writable_stack_pop_tags_update:
-  assumes
-    "pop_tags r s = s'"
-    "the_ptr (pointer r) < length (tags s)"
-    "writable_stack (tag r) ((tags s) ! the_ptr (pointer r))"
-  shows "writable_stack (tag r) ((tags s') ! the_ptr (pointer r))"
-  sorry
+lemma writable_stack_pop_tags_stack:
+  "writable_stack t stack \<Longrightarrow> writable_stack t (pop_tags_stack t stack)"
+proof (induction stack)
+  case Nil
+  then show ?case by simp
+next
+  case (Cons entry stack)
+  then show ?case using writable_stack.elims(2) by fastforce
+qed
 
 fun writable :: "tagged_ref \<Rightarrow> 'a globals_ram_scheme \<Rightarrow> bool" where
   "writable r s =
@@ -674,10 +673,9 @@ fun writable :: "tagged_ref \<Rightarrow> 'a globals_ram_scheme \<Rightarrow> bo
 lemma writable_update[simp]: "writable r (memwrite r' v s) = writable r s"
   by simp
 
-lemma writable_invalidated[intro]: "writable r s \<Longrightarrow> writable r (pop_tags r s)"
-  apply (simp add: Let_def)
-  apply auto
-  by (metis dropWhile_in list_update_beyond not_le nth_list_updateeq)
+lemma pop_tags_writable[intro]: "\<lbrakk>writable r s; wf_heap s\<rbrakk> \<Longrightarrow> writable r (pop_tags r s)"
+  apply (auto simp del: pop_tags_stack.simps)
+  by (metis nth_list_update_eq writable_stack_pop_tags_stack)
 
 fun new_pointer :: "'a globals_ram_scheme \<Rightarrow> pointer" where
   "new_pointer s = ptr_val (length (memory s))"
@@ -687,7 +685,9 @@ fun heap_new :: "val \<Rightarrow> 'a globals_ram_scheme \<Rightarrow> tagged_re
     (let p = new_pointer s;
          t = new_tag s in
     (\<lparr> pointer = p, tag = t \<rparr>,
-     s\<lparr> memory := memory s @ [v], tags := tags s @ [[t]], issued_tags := t # issued_tags s \<rparr>))"
+     s\<lparr> memory := memory s @ [v],
+        tags := tags s @ [[(Unique, {t})]],
+        issued_tags := t # issued_tags s \<rparr>))"
 
 fun_cases heap_new_elims: "heap_new v s = (r, s')"
 
@@ -697,22 +697,230 @@ lemma heap_new_writable: "\<lbrakk>wf_heap s; heap_new v s = (r', s')\<rbrakk> \
 
 lemma heap_new_wf_heap_update: "\<lbrakk>wf_heap s; heap_new v s = (r', s')\<rbrakk> \<Longrightarrow> wf_heap s'"
   apply (erule heap_new_elims)
-  by (auto simp add: Let_def)
+  by (auto simp add: Let_def wf_tags_snoc BorrowRoot)
 
-fun reborrow :: "tagged_ref \<Rightarrow> 'a globals_ram_scheme \<Rightarrow> tagged_ref * 'a globals_ram_scheme" where
-  "reborrow r s =
+fun reborrow_stack :: "ref_kind \<Rightarrow> tag \<Rightarrow> (ref_kind * tag set) stack \<Rightarrow> (ref_kind * tag set) stack"
+  where
+  (* reborrwing Unique *)
+  "reborrow_stack Unique t ((Unique, ts) # stack) = (Unique, {t}) # (Unique, ts) # stack" |
+  "reborrow_stack Unique t ((SharedReadWrite, ts) # stack) =
+    (Unique, {t}) # (SharedReadWrite, ts) # stack" |
+  (* reborrowing SharedReadWrite *)
+  "reborrow_stack SharedReadWrite t ((Unique, ts) # stack) =
+    (SharedReadWrite, {t}) # (Unique, ts) # stack" |
+  "reborrow_stack SharedReadWrite t ((SharedReadWrite, ts) # stack) =
+    (SharedReadWrite, insert t ts) # stack" |
+  (* reborrwing SharedReadOnly *)
+  "reborrow_stack SharedReadOnly t ((Unique, ts) # stack) =
+    (SharedReadOnly, {t}) # (Unique, ts) # stack" |
+  "reborrow_stack SharedReadOnly t ((SharedReadWrite, ts) # stack) =
+    (SharedReadOnly, {t}) # (SharedReadWrite, ts) # stack" |
+  "reborrow_stack SharedReadOnly t ((SharedReadOnly, ts) # stack) =
+    (SharedReadOnly, insert t ts) # stack" |
+  (* other cases are uninteresting as reborrow is not well-formed *)
+  "reborrow_stack _ _ [] = []" |
+  "reborrow_stack Unique _ ((SharedReadOnly, _) # stack) = []" |
+  "reborrow_stack SharedReadWrite _ ((SharedReadOnly, _) # stack) = []"
+
+lemma reborrow_stack_hd:
+  assumes
+    "reborrow_stack r t stack = stack'"
+    "stack' \<noteq> []"
+  shows "r = fst (hd stack') \<and> t \<in> snd (hd stack')"
+using assms proof (cases rule: reborrow_stack.elims)
+qed auto
+
+fun_cases reborrow_stack_elims_Unique[case_names _ UniqueUnique UniqueSRW]:
+  "reborrow_stack Unique t stack = (Unique, ts) # stack'"
+fun_cases reborrow_stack_elims_SRW[case_names _ SRWUnique SRWSRW]:
+  "reborrow_stack SharedReadWrite t stack = (SharedReadWrite, ts) # stack'"
+fun_cases reborrow_stack_elims_SRO[case_names _ SROUnique SROSRW SROSRO]:
+  "reborrow_stack SharedReadOnly t stack = (SharedReadOnly, ts) # stack'"
+
+lemma wf_reborrow_reborrow_stack_Unique:
+  assumes
+    "wf_reborrow stack"
+    "t \<notin> collect_tags_stack stack"
+    "reborrow_stack Unique t stack = stack'"
+    "stack' \<noteq> []"
+  shows "wf_reborrow stack'"
+proof -
+  have p: "Unique = fst (hd stack') \<and> t \<in> snd (hd stack')"
+    using assms reborrow_stack_hd by simp
+  then obtain ts rest where
+    q: "stack' = (Unique, ts) # rest"
+    using assms by (metis list.collapse prod.collapse)
+  then have "wf_reborrow ((Unique, ts) # rest)"
+  proof (cases t stack ts rest rule: reborrow_stack_elims_Unique)
+    case _
+    then show ?case using assms(3) q by blast
+  next
+    case (UniqueUnique ts' stack)
+    moreover obtain t' where
+      "ts' = {t'}"
+      using assms(1) calculation(1) unique_ref_head by blast
+    moreover have "wf_reborrow ((Unique, {t}) # (Unique, {t'}) # stack)"
+    proof (rule ReborrowUniqueUnique)
+      show "wf_reborrow ((Unique, {t'}) # stack)"
+        using assms(1) calculation(1) calculation(4) by auto
+    next
+      have "t \<notin> {t'} \<union> collect_tags_stack stack"
+        using assms(2) calculation(1) calculation(4) by auto
+      then show "t \<notin> insert t' (collect_tags_stack stack)" by simp
+    qed
+    ultimately show ?thesis by simp
+  next
+    case (UniqueSRW ts' stack)
+    moreover have "wf_reborrow ((Unique, {t}) # (SharedReadWrite, ts') # stack)"
+    proof (rule ReborrowSRWUnique)
+      show "wf_reborrow ((SharedReadWrite, ts') # stack)"
+        using assms(1) calculation(1) by blast
+    next
+      show "t \<notin> ts' \<union> collect_tags_stack stack"
+        using assms(2) calculation(1) by auto
+    qed
+    ultimately show ?thesis by simp
+  qed
+  then show ?thesis by (simp add: q)
+qed
+
+lemma wf_reborrow_reborrow_stack_SRW:
+  assumes
+    "wf_reborrow stack"
+    "t \<notin> collect_tags_stack stack"
+    "reborrow_stack SharedReadWrite t stack = stack'"
+    "stack' \<noteq> []"
+  shows "wf_reborrow stack'"
+proof -
+  have p: "SharedReadWrite = fst (hd stack') \<and> t \<in> snd (hd stack')"
+    using assms reborrow_stack_hd by simp
+  then obtain ts rest where
+    q: "stack' = (SharedReadWrite, ts) # rest"
+    using assms by (metis list.collapse prod.collapse)
+  then have "wf_reborrow ((SharedReadWrite, ts) # rest)"
+  proof (cases t stack ts rest rule: reborrow_stack_elims_SRW)
+    case _
+    then show ?case using assms(3) q by blast
+  next
+    case (SRWUnique ts' stack)
+    moreover obtain t' where
+      "ts' = {t'}"
+      using assms(1) calculation(1) unique_ref_head by blast
+    moreover have "wf_reborrow ((SharedReadWrite, {t}) # (Unique, {t'}) # stack)"
+    proof (rule ReborrowUniqueSRW)
+      show "wf_reborrow ((Unique, {t'}) # stack)"
+        using assms SRWUnique calculation by simp
+    next
+      have "t \<notin> {t'} \<union> (collect_tags_stack stack)"
+        using assms(2) calculation(1) calculation(4) by auto
+      then show "t \<notin> insert t' (collect_tags_stack stack)" by auto
+    qed
+    moreover have "wf_reborrow ((SharedReadWrite, ts) # (Unique, ts') # stack)"
+      using calculation by simp
+    ultimately show ?thesis by simp
+  next
+    case (SRWSRW ts')
+    moreover have "wf_reborrow ((SharedReadWrite, insert t ts') # rest)"
+    proof (rule ReborrowSRWSRW)
+      show "wf_reborrow ((SharedReadWrite, ts') # rest)" using assms SRWSRW by simp
+    next
+      show "t \<notin> ts' \<union> collect_tags_stack rest" using assms SRWSRW by simp
+    qed
+    ultimately show ?thesis by simp
+  qed
+  then show ?thesis by (simp add: q)
+qed
+
+lemma wf_reborrow_reborrow_stack_SRO:
+  assumes
+    "wf_reborrow stack"
+    "t \<notin> collect_tags_stack stack"
+    "reborrow_stack SharedReadOnly t stack = stack'"
+    "stack' \<noteq> []"
+  shows "wf_reborrow stack'"
+proof -
+  have p: "SharedReadOnly = fst (hd stack') \<and> t \<in> snd (hd stack')"
+    using assms reborrow_stack_hd by simp
+  then obtain ts rest where
+    q: "stack' = (SharedReadOnly, ts) # rest"
+    using assms by (metis list.collapse prod.collapse)
+  then have "wf_reborrow ((SharedReadOnly, ts) # rest)"
+  proof (cases t stack ts rest rule: reborrow_stack_elims_SRO)
+    case _
+    then show ?case using assms(3) q by blast
+  next
+    case (SROUnique ts' stack)
+    moreover obtain t' where
+      "ts' = {t'}"
+      using assms(1) calculation(1) unique_ref_head by blast
+    moreover have "wf_reborrow ((SharedReadOnly, {t}) # (Unique, {t'}) # stack)"
+    proof (rule ReborrowUniqueSRO)
+      show "wf_reborrow ((Unique, {t'}) # stack)"
+        using assms calculation by simp
+    next
+      have "t \<notin> {t'} \<union> collect_tags_stack stack"
+        using assms(2) calculation(1) calculation(4) by auto
+      then show "t \<notin> insert t' (collect_tags_stack stack)" by simp
+    qed
+    ultimately show ?thesis by (simp add: q)
+  next
+    case (SROSRW ts' stack)
+    moreover have "wf_reborrow ((SharedReadOnly, {t}) # (SharedReadWrite, ts') # stack)"
+    proof (rule ReborrowSRWSRO)
+      show "wf_reborrow ((SharedReadWrite, ts') # stack)"
+        using assms(1) calculation(1) by auto
+    next
+      show "t \<notin> ts' \<union> collect_tags_stack stack"
+        using assms(2) calculation(1) by fastforce
+    qed
+    ultimately show ?thesis by (simp add: q)
+  next
+    case (SROSRO ts')
+    moreover have "wf_reborrow ((SharedReadOnly, insert t ts') # rest)"
+    proof (rule ReborrowSROSRO)
+      show "wf_reborrow ((SharedReadOnly, ts') # rest)"
+        using assms(1) calculation(1) by blast
+    next
+      show "t \<notin> ts' \<union> collect_tags_stack rest" using assms SROSRO by simp
+    qed
+    ultimately show ?thesis by simp
+  qed
+  then show ?thesis by (simp add: q)
+qed
+
+
+lemma wf_reborrow_reborrow_stack:
+  assumes
+    "wf_reborrow stack"
+    "t \<notin> collect_tags_stack stack"
+    "reborrow_stack k t stack = stack'"
+    "stack' \<noteq> []"
+  shows "wf_reborrow stack'"
+proof (cases k)
+  case Unique
+  then show ?thesis using assms wf_reborrow_reborrow_stack_Unique by simp
+next
+  case SharedReadWrite
+  then show ?thesis using assms wf_reborrow_reborrow_stack_SRW by simp
+next
+  case SharedReadOnly
+  then show ?thesis using assms wf_reborrow_reborrow_stack_SRO by simp
+qed
+
+fun reborrow :: "ref_kind \<Rightarrow> tagged_ref \<Rightarrow> 'a globals_ram_scheme \<Rightarrow> tagged_ref * 'a globals_ram_scheme" where
+  "reborrow k r s =
     (let p = the_ptr (pointer r) in
     let t = new_tag s in
-    let tags = (tags s)[p := t # ((tags s) ! p)] in
-    (\<lparr> pointer = pointer r, tag = t \<rparr>, s\<lparr> tags := tags, issued_tags := t # issued_tags s \<rparr>))"
+    let tags = (tags s)[p := reborrow_stack k (tag r) ((tags s) ! p)] in
+    (\<lparr> pointer = pointer r, tag = t \<rparr>,  s\<lparr> tags := tags, issued_tags := t # issued_tags s \<rparr>))"
 
-fun_cases reborrow_elims: "reborrow r s = (r', s')"
+fun_cases reborrow_elims: "reborrow k r s = (r', s')"
 
-lemma reborrow_pointer: "reborrow r s = (r', s') \<Longrightarrow> pointer r' = pointer r"
+lemma reborrow_pointer: "reborrow k r s = (r', s') \<Longrightarrow> pointer r' = pointer r"
   apply (erule reborrow_elims)
   by (auto simp: Let_def)
 
-lemma reborrow_update_heap: "\<lbrakk>wf_heap s; writable r s; reborrow r s = (r', s')\<rbrakk> \<Longrightarrow> wf_heap s'"
+lemma reborrow_update_heap: "\<lbrakk>wf_heap s; writable r s; reborrow k r s = (r', s')\<rbrakk> \<Longrightarrow> wf_heap s'"
   apply (erule reborrow_elims)
   apply (auto simp add: Let_def)
   using wf_tags_update apply simp
